copy substitution lemmas from max-ctx-growth-ip-pr-muDot to max-ctx-size-ip-pr-muDot

dev/expansion/max-ctx-size-ip-pr-muDot.v
@@ -225,6 +225,8 @@ with fv_defs(ds: defs) : vars :=
   | defs_cons n d tl => (fv_def d) \u (fv_defs tl)
   end.
 
+Definition fv_ctx_types(G: ctx): vars := (fv_in_values (fun T => fv_typ T) G).
+
 
 (* ###################################################################### *)
 (** ** Operational Semantics *)
@@ -707,6 +709,8 @@ Proof.
   intros x y. apply typ_mutind; intros; simpls; f_equal*. apply* subst_fresh_pth.
 Qed.
 
+Definition subst_fresh_typ(x y: var) := proj1 (subst_fresh_typ_dec_decs x y).
+
 Lemma subst_fresh_trm_def_defs: forall x y,
   (forall t : trm , x \notin fv_trm  t  -> subst_trm  x y t  = t ) /\
   (forall d : def , x \notin fv_def  d  -> subst_def  x y d  = d ) /\
@@ -716,6 +720,34 @@ Proof.
   + apply* subst_fresh_avar.
   + apply* subst_fresh_typ_dec_decs.
   + apply* subst_fresh_avar.
+Qed.
+
+Lemma invert_fv_ctx_types_push: forall x z T G,
+  x \notin fv_ctx_types (G & z ~ T) -> x \notin fv_typ T /\ x \notin (fv_ctx_types G).
+Proof.
+  introv N.
+  unfold fv_ctx_types in *.
+  unfold fv_in_values in *.
+  rewrite <- cons_to_push in *.
+  rewrite values_def in *.
+  unfold LibList.map in *.
+  do 2 rewrite LibList.fold_right_cons in *.
+  simpl in *.
+  apply notin_union in N. exact N.
+Qed.
+
+Lemma subst_fresh_ctx: forall x y G,
+  x \notin fv_ctx_types G -> subst_ctx x y G = G.
+Proof.
+  intros x y.
+  apply (env_ind (fun G => x \notin fv_ctx_types G -> subst_ctx x y G = G)).
+  + intro N. unfold subst_ctx. apply map_empty.
+  + intros G z T IH N.
+    apply invert_fv_ctx_types_push in N. destruct N as [N1 N2].
+    unfold subst_ctx in *. rewrite map_push.
+    rewrite (IH N2).
+    rewrite (subst_fresh_typ _ _ N1).
+    reflexivity.
 Qed.
 
 Definition subst_fvar(x y z: var): var := If x = z then y else z.
@@ -1173,6 +1205,22 @@ Proof.
     - apply* IHHdsDs.
 Qed.
 
+Lemma invert_ty_var: forall G x T,
+  ty_trm G (trm_var (avar_f x)) T ->
+  exists T' n, subtyp ip oktrans G T' T n /\ binds x T' G.
+Proof.
+  introv Ty. gen_eq t: (trm_var (avar_f x)). gen x.
+  induction Ty; intros x' Eq; try (solve [ discriminate ]).
+  + inversions Eq. exists T (ctx_size G).
+    apply (conj (subtyp_tmode (subtyp_refl _ _ _))). assumption.
+  + subst. specialize (IHTy _ eq_refl). destruct IHTy as [T' [n2 [St Bi]]].
+    exists T' (max n n2). split.
+    - apply subtyp_trans with T.
+      * refine (subtyp_ctx_size _ St). apply Max.le_max_r.
+      * refine (subtyp_ctx_size _ H). apply Max.le_max_l.
+    - exact Bi.
+Qed.
+
 Lemma invert_ty_mtd_inside_ty_defs: forall G ds Ds m S T body,
   ty_defs G ds Ds ->
   defs_has ds (label_mtd m) (def_mtd body) ->
@@ -1608,7 +1656,6 @@ Proof.
   apply (W d eq_refl Hle Ok).
 Qed.
 
-(*
 Lemma weaken_ty_trm_end: forall G1 G2 e T,
   ok (G1 & G2) -> ty_trm G1 e T -> ty_trm (G1 & G2) e T.
 Proof.
@@ -1618,6 +1665,7 @@ Proof.
   apply (W (G1 & empty)); rewrite* concat_empty_r.
 Qed.
 
+(*
 Lemma weaken_ty_def_end: forall G1 G2 i d,
   ok (G1 & G2) -> ty_def G1 i d -> ty_def (G1 & G2) i d.
 Proof.
@@ -1678,6 +1726,7 @@ Note that in general, u is a term, but for our purposes, it suffices to consider
 the special case where u is a variable.
 *)
 
+
 Lemma subst_label_for_dec: forall n x y D,
   label_for_dec n (subst_dec x y D) = label_for_dec n D.
 Proof.
@@ -1712,33 +1761,68 @@ Inductive tyvar: pmode -> ctx -> var -> typ -> Prop :=
       ty_trm G (trm_var (avar_f x)) T ->
       tyvar ip G x T.
 
-(*
+(* TODO doesn't hold as such, we need some wf-ness as well *)
+Lemma middle_notin: forall G1 x S G2,
+  ok (G1 & x ~ S & G2) ->
+  x # G1 /\
+  x \notin fv_ctx_types G1 /\
+  x \notin fv_typ S /\
+  x \notin dom G2.
+Admitted.
+
+Lemma ok_concat_binds_left_to_notin_right: forall (A: Type) y (S: A) G1 G2,
+  ok (G1 & G2) -> binds y S G1 -> y # G2.
+Admitted.
+
+Lemma concat_subst_ctx: forall x y G1 G2,
+  subst_ctx x y G1 & subst_ctx x y G2 = subst_ctx x y (G1 & G2).
+Proof.
+  intros. unfold subst_ctx. rewrite map_concat. reflexivity.
+Qed.
+
+(* TODO also need x <> z *)
+Lemma subst_dec_preserves_clo: forall D x y,
+  (forall z : var, open_dec z D = D) ->
+  (forall z : var, open_dec z (subst_dec x y D) = subst_dec x y D).
+Admitted.
+
+Lemma subst_ctx_preserves_notin: forall x y z G,
+  z # G -> z # (subst_ctx x y G).
+  (* because subst_ctx only modifies rhs, not lhs of bindings *)
+Admitted.
+
+Lemma subst_decs_preserves_cbounds: forall x y Ds,
+  cbounds_decs Ds -> cbounds_decs (subst_decs x y Ds).
+Admitted.
+
+Axiom okadmit: forall G: ctx, ok G.
+
 Lemma subst_principles: forall y S,
    (forall m G T Ds, exp m G T Ds -> forall G1 G2 x,
      G = G1 & x ~ S & G2 ->
      tyvar m G1 y S ->
      ok (G1 & x ~ S & G2) ->
-     exp ip (G1 & (subst_ctx x y G2)) (subst_typ x y T) (subst_decs x y Ds))
+     exp m (G1 & (subst_ctx x y G2)) (subst_typ x y T) (subst_decs x y Ds))
 /\ (forall m G t l D, has m G t l D -> forall G1 G2 x,
      G = (G1 & (x ~ S) & G2) ->
      tyvar m G1 y S ->
      ok (G1 & (x ~ S) & G2) ->
-     has ip (G1 & (subst_ctx x y G2)) (subst_trm x y t) l (subst_dec x y D))
+     has m (G1 & (subst_ctx x y G2)) (subst_trm x y t) l (subst_dec x y D))
 /\ (forall m1 m2 G T U n, subtyp m1 m2 G T U n -> forall G1 G2 x,
      G = (G1 & (x ~ S) & G2) ->
      tyvar m1 G1 y S ->
      ok (G1 & (x ~ S) & G2) ->
-     subtyp ip m2 (G1 & (subst_ctx x y G2)) (subst_typ x y T) (subst_typ x y U))
+     subtyp m1 m2 (G1 & (subst_ctx x y G2)) (subst_typ x y T) (subst_typ x y U) n)
 /\ (forall m G D1 D2 n, subdec m G D1 D2 n -> forall G1 G2 x,
      G = (G1 & (x ~ S) & G2) ->
      tyvar m G1 y S ->
      ok (G1 & (x ~ S) & G2) ->
-     subdec ip (G1 & (subst_ctx x y G2)) (subst_dec x y D1) (subst_dec x y D2))
+     subdec m (G1 & (subst_ctx x y G2)) (subst_dec x y D1) (subst_dec x y D2) n)
 /\ (forall m G Ds1 Ds2 n, subdecs m G Ds1 Ds2 n -> forall G1 G2 x,
      G = (G1 & (x ~ S) & G2) ->
      tyvar m G1 y S ->
      ok (G1 & (x ~ S) & G2) ->
-     subdecs ip (G1 & (subst_ctx x y G2)) (subst_decs x y Ds1) (subst_decs x y Ds2))
+     subdecs m (G1 & (subst_ctx x y G2)) (subst_decs x y Ds1) (subst_decs x y Ds2) n)
 /\ (forall G t T, ty_trm G t T -> forall G1 G2 x,
      G = (G1 & (x ~ S) & G2) ->
      tyvar ip G1 y S ->
@@ -1761,24 +1845,24 @@ Proof.
   (* case exp_bind *)
   + intros. simpl. apply exp_bind.
   (* case exp_sel *)
-  + intros m G v L Lo Hi Ds Has IHHas Exp IHExp G1 G2 x Eqm EqG Tyy Ok. subst.
-    specialize (IHHas _ _ _ eq_refl eq_refl Tyy Ok).
-    specialize (IHExp _ _ _ eq_refl eq_refl Tyy Ok).
+  + intros m G v L Lo Hi Ds Has IHHas Exp IHExp G1 G2 x EqG Tyy Ok. subst.
+    specialize (IHHas _ _ _ eq_refl Tyy Ok).
+    specialize (IHExp _ _ _ eq_refl Tyy Ok).
     unfold subst_typ. unfold subst_pth. unfold subst_avar. case_if.
     - simpl in IHHas. case_if.
       apply (exp_sel IHHas IHExp).
     - simpl in IHHas. case_if.
       apply (exp_sel IHHas IHExp).
   + (* case has_trm *)
-    intros G t T Ds l D Ty IHTy Exp IHExp Has Clo G1 G2 x Eqm EqG Bi Ok.
+    intros G t T Ds l D Ty IHTy Exp IHExp Has Clo G1 G2 x EqG Bi Ok.
     subst. specialize (IHTy _ _ _ eq_refl Bi Ok).
     apply has_trm with (subst_typ x y T) (subst_decs x y Ds).
     - exact IHTy.
     - apply* IHExp.
     - apply* subst_decs_has.
-    - intro z. specialize (Clo z). admit.
+    - apply (subst_dec_preserves_clo _ _ Clo).
   + (* case has_var *)
-    intros G z T Ds l D Ty IHTy Exp IHExp Has G1 G2 x Eqm EqG Bi Ok.
+    intros G z T Ds l D Ty IHTy Exp IHExp Has G1 G2 x EqG Bi Ok.
     subst. specialize (IHTy _ _ _ eq_refl Bi Ok). simpl in *. case_if.
     - (* case z = x *)
       rewrite (subst_open_commute_dec x y x D). unfold subst_fvar. case_if.
@@ -1793,81 +1877,111 @@ Proof.
       * apply* IHExp.
       * apply (subst_decs_has x y Has).
   + (* case has_pr *)
-    intros. discriminate.
+    intros G z T Ds l D Bi Exp IHExp DsHas G1 G2 x EqG Ty Ok. subst. simpl in *.
+    destruct (middle_notin Ok) as [N1 [N2 [N3 N4]]].
+    case_if.
+    - (* case z = x *)
+      rewrite (subst_open_commute_dec x y x D). unfold subst_fvar. case_if.
+      lets Eq: (binds_middle_eq_inv Bi Ok). subst T.
+      inversion Ty; subst.
+      apply has_pr with (subst_typ x y S) (subst_decs x y Ds).
+      * rewrite (subst_fresh_typ _ _ N3).
+        apply (binds_concat_left H).
+        apply ok_remove in Ok.
+        unfold subst_ctx.
+        rewrite dom_map.
+        apply (ok_concat_binds_left_to_notin_right Ok H).
+      * apply* IHExp.
+      * apply (subst_decs_has x y DsHas).
+    - (* case z <> x *)
+      rewrite (subst_open_commute_dec x y z D). unfold subst_fvar. case_if.
+      apply has_pr with (subst_typ x y T) (subst_decs x y Ds).
+      * lets Bi': (binds_subst Bi H).
+        rewrite <- (subst_fresh_ctx y G1 N2).
+        rewrite -> (concat_subst_ctx _ _).
+        apply (subst_binds _ _ Bi').
+      * apply* IHExp.
+      * apply (subst_decs_has x y DsHas).
   + (* case subtyp_refl *)
-    intros m G v L Lo Hi Has IHHas G1 G2 x Eqm EqG Tyy Ok. subst.
-    specialize (IHHas _ _ _ eq_refl eq_refl Tyy Ok).
-    unfold subst_dec in IHHas. fold subst_typ in IHHas.
-    unfold subst_trm, subst_avar in IHHas.
-    simpl. case_if; apply (subtyp_refl IHHas).
+    introv EqG Ty Ok. subst. admit. (* TODO trivial *)
   + (* case subtyp_top *)
-    intros. simpl. apply subtyp_top.
+    intros. simpl. subst.  admit. (* TODO trivial *)
   + (* case subtyp_bot *)
-    intros. simpl. apply subtyp_bot.
+    intros. simpl. subst.  admit. (* TODO trivial *)
   + (* case subtyp_bind *)
-    intros L m G Ds1 Ds2 Sds IH G1 G2 x Eqm EqG Bi Ok. subst.
+    intros L m G Ds1 Ds2 n Sds IH G1 G2 x EqG Bi Ok. subst.
     apply_fresh subtyp_bind as z. fold subst_decs.
     assert (zL: z \notin L) by auto.
     specialize (IH z zL G1 (G2 & z ~ typ_bind Ds1) x).
     rewrite concat_assoc in IH.
-    specialize (IH eq_refl eq_refl Bi).
+    specialize (IH eq_refl Bi).
     unfold subst_ctx in IH. rewrite map_push in IH. simpl in IH.
     rewrite concat_assoc in IH.
     rewrite (subst_open_commute_decs x y z Ds1) in IH.
     rewrite (subst_open_commute_decs x y z Ds2) in IH.
     unfold subst_fvar in IH.
     assert (x <> z) by auto. case_if.
-    unfold subst_ctx. apply IH. admit.
+    unfold subst_ctx. apply IH. apply okadmit.
   + (* case subtyp_sel_l *)
-    intros m G v L Lo Hi T Has IHHas St IHSt G1 G2 x Eqm EqG Bi Ok. subst.
-    specialize (IHSt _ _ _ eq_refl eq_refl Bi Ok).
-    specialize (IHHas _ _ _ eq_refl eq_refl Bi Ok).
+    intros m G v L Lo Hi T n Has IHHas St IHSt G1 G2 x EqG Bi Ok. subst.
+    specialize (IHSt _ _ _ eq_refl Bi Ok).
+    specialize (IHHas _ _ _ eq_refl Bi Ok).
     simpl in *.
     case_if; apply (subtyp_sel_l IHHas IHSt).
   + (* case subtyp_sel_r *)
-    intros m G v L Lo Hi T Has IHHas St1 IHSt1 St2 IHSt2 G1 G2 x Eqm EqG Bi Ok. subst.
-    specialize (IHSt1 _ _ _ eq_refl eq_refl Bi Ok).
-    specialize (IHSt2 _ _ _ eq_refl eq_refl Bi Ok).
-    specialize (IHHas _ _ _ eq_refl eq_refl Bi Ok).
+    intros m G v L Lo Hi T n Has IHHas St1 IHSt1 St2 IHSt2 G1 G2 x EqG Bi Ok. subst.
+    specialize (IHSt1 _ _ _ eq_refl Bi Ok).
+    specialize (IHSt2 _ _ _ eq_refl Bi Ok).
+    specialize (IHHas _ _ _ eq_refl Bi Ok).
     simpl in *.
     case_if; apply (subtyp_sel_r IHHas IHSt1 IHSt2).
   + (* case subtyp_tmode *)
-    intros m G T1 T2 St IH G1 G2 x Eqm EqG Bi Ok. subst.
-    specialize (IH _ _ _ eq_refl eq_refl Bi Ok).
+    intros m G T1 T2 n St IH G1 G2 x EqG Bi Ok. subst.
+    specialize (IH _ _ _ eq_refl Bi Ok).
     apply (subtyp_tmode IH).
   + (* case subtyp_trans *)
     intros m G T1 T2 T3 St12 IH12 St23 IH23 G1 G2 x Eqm EqG Bi Ok. subst.
     apply* subtyp_trans.
+  + (* case subtyp_ctx_size *)
+    intros. subst. apply* subtyp_ctx_size.
   + (* case subdec_typ *)
-    intros. apply* subdec_typ.
+    intros. subst. apply* subdec_typ.
   + (* case subdec_fld *)
     intros. apply* subdec_fld.
   + (* case subdec_mtd *)
     intros. apply* subdec_mtd.
   + (* case subdecs_empty *)
-    intros. apply subdecs_empty.
+    intros. subst. apply subdecs_empty. admit. (* TODO trivial *)
   + (* case subdecs_push *)
-    intros m G n Ds1 Ds2 D1 D2 Has Sd IH1 Sds IH2 G1 G2 x Eq1 Eq2 Bi Ok. subst.
-    specialize (IH1 _ _ _ eq_refl eq_refl Bi Ok).
-    specialize (IH2 _ _ _ eq_refl eq_refl Bi Ok).
+    intros m G n Ds1 Ds2 D1 D2 n1 Has Sd IH1 Sds IH2 G1 G2 x Eq1 Bi Ok. subst.
+    specialize (IH1 _ _ _ eq_refl Bi Ok).
+    specialize (IH2 _ _ _ eq_refl Bi Ok).
     apply (subst_decs_has x y) in Has.
     rewrite <- (subst_label_for_dec n x y D2) in Has.
     apply subdecs_push with (subst_dec x y D1); 
       fold subst_dec; fold subst_decs; assumption.
+  + (* case subdecs_refl *)
+    introv Hle EqG Ty Ok. apply subdecs_refl. subst. admit. (* TODO trivial *)
   + (* case ty_var *)
-    intros G z T Biz G1 G2 x EqG Biy Ok.
-    subst G. unfold subst_trm, subst_avar. case_var.
+    intros G z T Biz G1 G2 x EqG Tyy Ok. subst G.
+    destruct (middle_notin Ok) as [xG1 [N2 [N3 N4]]].
+    unfold subst_trm, subst_avar. case_var.
     - (* case z = x *)
       assert (EqST: T = S) by apply (binds_middle_eq_inv Biz Ok). subst.
-      assert (yG2: y # (subst_ctx x y G2)) by admit.
-      assert (xG1: x # G1) by admit.
-      assert (Eq: (subst_typ x y S) = S) by admit.
-      rewrite Eq. 
+      inversions Tyy. rename H into Tyy.
+      lets Ty: (invert_ty_var Tyy).
+      destruct Ty as [S' [n [St Biy]]].
+      lets yG2: (ok_concat_binds_left_to_notin_right (ok_remove Ok) Biy).
+      apply (@subst_ctx_preserves_notin x y y G2) in yG2.
       apply weaken_ty_trm_end.
       * unfold subst_ctx. auto.
-      * assumption.
+      * rewrite (@subst_fresh_typ x y S N3). exact Tyy.
     - (* case z <> x *)
-      apply ty_var. admit. (* TODO! *)
+      apply ty_var.
+      rewrite <- (subst_fresh_ctx y G1 N2).
+      rewrite -> (concat_subst_ctx _ _).
+      lets Bi': (binds_subst Biz C).
+      apply (subst_binds _ _ Bi').
   (* case ty_sel *)
   + intros G t l T Has IH G1 G2 x Eq Bi Ok. apply* ty_sel.
   (* case ty_call *)
@@ -1888,10 +2002,10 @@ Proof.
       specialize (IHTyds eq_refl Bi).
       unfold subst_ctx in IHTyds. rewrite map_push in IHTyds. unfold subst_ctx.
       apply IHTyds. auto.
-    - admit. (* TODO holds *)
+    - apply (subst_decs_preserves_cbounds _ _ Cb).
   (* case ty_sbsm *)
-  + intros G t T U Ty IHTy St IHSt G1 G2 x Eq Bi Ok. subst.
-    apply ty_sbsm with (subst_typ x y T).
+  + intros G t T U n Ty IHTy St IHSt G1 G2 x Eq Bi Ok. subst.
+    apply ty_sbsm with (subst_typ x y T) n.
     - apply* IHTy.
     - apply* IHSt.
   (* case ty_typ *)
@@ -1928,19 +2042,35 @@ Proof.
   specialize (P _ t T tTy G empty x).
   unfold subst_ctx in P. rewrite map_empty in P.
   repeat (progress (rewrite concat_empty_r in P)).
+  apply tyvar_ip in yTy.
   apply* P.
 Qed.
 
-Lemma subdecs_subst_principle: forall G x y S Ds1 Ds2,
+Lemma pr_subdec_subst_principle: forall G x y S D1 D2 n,
   ok (G & x ~ S) ->
-  subdecs ip (G & x ~ S) Ds1 Ds2 ->
-  ty_trm G (trm_var (avar_f y)) S ->
-  subdecs ip G (subst_decs x y Ds1) (subst_decs x y Ds2).
+  subdec pr (G & x ~ S) D1 D2 n ->
+  binds y S G ->
+  subdec pr G (subst_dec x y D1) (subst_dec x y D2) n.
 Proof.
-  introv Hok Sds yTy. destruct (subst_principles y S) as [_ [_ [_ [_ [P _]]]]].
-  specialize (P _ _ Ds1 Ds2 Sds G empty x).
+  introv Hok Sd yTy. destruct (subst_principles y S) as [_ [_ [_ [P _]]]].
+  specialize (P _ _ D1 D2 _ Sd G empty x).
   unfold subst_ctx in P. rewrite map_empty in P.
   repeat (progress (rewrite concat_empty_r in P)).
+  apply tyvar_pr in yTy.
+  apply* P.
+Qed.
+
+Lemma subdecs_subst_principle: forall G x y S Ds1 Ds2 n,
+  ok (G & x ~ S) ->
+  subdecs ip (G & x ~ S) Ds1 Ds2 n ->
+  ty_trm G (trm_var (avar_f y)) S ->
+  subdecs ip G (subst_decs x y Ds1) (subst_decs x y Ds2) n.
+Proof.
+  introv Hok Sds yTy. destruct (subst_principles y S) as [_ [_ [_ [_ [P _]]]]].
+  specialize (P _ _ Ds1 Ds2 _ Sds G empty x).
+  unfold subst_ctx in P. rewrite map_empty in P.
+  repeat (progress (rewrite concat_empty_r in P)).
+  apply tyvar_ip in yTy.
   apply* P.
 Qed.
 
@@ -1948,6 +2078,7 @@ Qed.
 (* ###################################################################### *)
 (** ** Narrowing *)
 
+(*
 Lemma narrow_ty_trm: forall G y T1 T2 u U,
   ok (G & y ~ T2) ->
   subtyp ip oktrans G T1 T2 ->
@@ -2370,8 +2501,6 @@ Axiom subsub2eq: forall m1 m2 G T1 T2,
   subtyp m1 m2 G T2 T1 ->
   T1 = T2.
 *)
-
-Axiom okadmit: forall G: ctx, ok G.
 
 (* env-grow restricted narrowing: Narrowing for derivations which grow the env by at
    most d entries *)
